proof/SystemF/Preservation.v
@@ -4,62 +4,103 @@ Require Import EvJudge.
 Require Import SubValueValue.
 Require Import SubTypeValue.
 
+(** Well formed expresions don't have type binders that shadow
+    other variables. 
+    TODO: Still have to show that when eval takes a step, can get
+          the resulting term back to a well formed one.
+**)
+Inductive wellformedX : exp -> Prop :=
+ | WFX_var
+   :  forall v
+   ,  wellformedX (XVar v)
+
+ | WFX_lam
+   :  forall x T1 t2
+   ,  wellformedX (XLam x T1 t2)
+
+ | WFX_app
+   : forall t1 t2
+   ,  wellformedX t1 
+   -> wellformedX t2
+   -> wellformedX (XApp t1 t2)
+
+ | WFX_LAM 
+   :  forall a t12
+   ,  ~bindsX a t12
+   -> wellformedX (XLAM a t12)
+
+ | WFX_APP
+   :  forall t1 T2
+   ,  wellformedX t1
+   -> wellformedX (XAPP t1 T2).
+
+Hint Constructors wellformedX.
+
 
 (* When a well typed term transitions to the next state, 
    its type is perserved.
  *)
 Theorem preservation
  :  forall kenv tenv t t' T
- ,  TYPE kenv tenv t  T
+ ,  closedX t -> wellformedX t
+ -> TYPE kenv tenv t  T
  -> STEP t t'
  -> TYPE kenv tenv t' T.
 Proof.
- intros kenv tenv t t' T Htype Hstep.
+ intros kenv tenv t t' T.
+ intros HcX HwX Htype Hstep.
  gen t' T.
- induction t; intros.
+ induction t. 
 
  Case "XVar". 
-  inversions Hstep.
+  intros. inversions Hstep.
 
  Case "XLam".
-  inversion Hstep.
+  intros. inversions Hstep.
 
  Case "XApp".
-  inversions Hstep.
+  intros. inversions Hstep.
   SCase "EVAppAbs".
-   inversions Htype.
-   eapply subst_value_value.
-    intro. 
-     apply values_are_closed in H2.
-     unfold closedX in H2.
-     specialize H2 with z. intro. contradiction.
-    inversion H4. eauto.
-    auto.
+   inversions Htype. inversions H4.
+   eapply subst_value_value; eauto.
   SCase "EVApp1".
-   inversions Htype. eauto.
+   inversions Htype.
+   eapply TYApp. apply IHt1.
+   eauto. inversions HwX. auto. auto. eauto. eauto.
+ eauto.
   SCase "EVApp2".
-   inversions Htype. eauto.
+   inversions Htype.
+   eapply TYApp. eauto. apply IHt2.
+   eauto. inversions HwX. auto. auto. auto.
 
  Case "XLAM".
-  inversions Hstep.
+  intros. inversions Hstep.
 
  Case "XAPP".
+  intros.
+  inversions HwX.
   inverts keep Hstep.
   inverts keep Htype. 
-  inverts keep H5. sort.
+  inverts keep H6.
   SCase "EVAPPLAM".
-   lets Hs: subst_type_value H10 H7.
-    auto. 
-     admit. (** fixme **)
-    auto.
+   lets Hs: subst_type_value H11 H8.
+    auto. auto. inversions H0. auto.
    eapply type_tyenv_invariance.
     apply Hs. eauto.
-    intros. sort.
+    intro. intro. intro. 
+      contradict H1.
+      lets C1: closedX_APP_elim1 HcX.
+      unfold closedX in C1. specialize C1 with x.
 
-   inversions H5.
-   eapply IHt.
-    eapply EVAPPLAM.
-    (* need that T2 is closed add to EVAPPABS *)
-   
+      assert (valname x -> freeX x (substTX a t0 t12) -> freeX x t12).
+       admit. (** easy: x cannot be in t0  **)
 
+      contradict C1. 
+      lets D1: H1 H C1.
+      apply FreeX_LAM. auto. auto.
+
+  SCase "t1 steps".
+   inversions Htype.
+   eapply TYAPP. auto. 
+   apply IHt; eauto. auto. 
 Qed.   
